$$
p_iV_i = nRT_i \\
p_i = \frac{nRT_i}{V_i} = \frac{nRT_i}{S_ix_i} \\
\begin{aligned}
  P_1 = P_2 \lrArr p_1S_1 = p_2S_2 \lrArr\frac{p_1}{p_2} = \frac{S_2}{S_1}
\end{aligned} \\
\lrArr \frac{S_2}{S_1} = \frac{p_1} {p_2} = \frac{S_2x_2}{S_1x_1}\frac{T_1}{T_2} = \frac{S_2x_2}{S_1x_1} \\
\begin{aligned}
  \lrArr x_1 = x_2 & \text{ Å¼e co?}
\end{aligned}

$$



$$
\begin{aligned}
  \Delta U = c_Vn\Delta T + nRT'\ln \frac{V_1'}{V_1} & ; & \Delta U = \frac{i}{2}nR\Delta T
\end{aligned} \\
c_Vn\Delta T + nRT'\ln \frac{V_1'}{V_1} = \frac{i}{2}nR\Delta T \\
nRT'\ln \frac{V_1'}{V_1} = n\Delta T [\frac{iR}{2} - c_V] \\
\ln \frac{V_1'}{V_1} = \frac{\Delta T}{RT'}[\frac{iR}{2} - c_V] \\
\frac{V_1'}{V_1} = e^{\frac{\Delta T}{RT'}[\frac{iR}{2} - c_V]} \\
S_1x_1' = V_1' = V_1 e^{\frac{\Delta T}{RT'}[\frac{iR}{2} - c_V]} \\
x_1' = x_1 e^{\frac{\Delta T}{RT'}[\frac{iR}{2} - c_V]} \\
$$  
   
  
   
$$
S_1p_{atm} + S_2p_2 - S_1p_1 - S_2p_{atm} = 0 \\
p_i = \frac{nRT}{x_iS_i} \\
S_1p_{atm} + \frac{nRT}{x_2} - \frac{nRT}{x_1} - S_2p_{atm} = 0 \\
\frac{1}{x_2} - \frac{1}{x_1} = \frac{p_{atm}[S_2-S_1]}{nRT} \\
\frac{1}{x_2 + \Delta x} - \frac{1}{x_1 - \Delta x} = \frac{2}{3} \frac{p_{atm}[S_2-S_1]}{nRT} = \frac{2}{3} [\frac{1}{x_2} - \frac{1}{x_1}]
$$

$$
\epsilon = -\frac{\partial (BS)}{\partial t} = -B\frac{\partial S}{\partial t} = -B \frac{\partial S}{\partial \theta} \omega
$$